Give layer impl translation for MailServer, state the big theorem.

src/Examples/MailServer/MailRefinement.v
@@ -8,3 +8,55 @@ From RecoveryRefinement Require AtomicPair.Helpers.
 From RecoveryRefinement.Goose Require Import Machine GoZeroValues Heap GoLayer.
 From RecoveryRefinement.Goose Require Import Machine.
 From RecoveryRefinement.Goose Require Import GoZeroValues.
+
+Inductive compile_mail_base {gm: GoModel} : forall {T}, proc Mail.Op T → proc GoLayer.Op T → Prop :=
+| cm_open :
+    compile_mail_base (Call Mail.Open)
+                      (MailServer.Open)
+| cm_pickup uid :
+    compile_mail_base (Mail.pickup uid)
+                      (MailServer.Pickup uid)
+| cm_deliver uid msg :
+    compile_mail_base (Mail.deliver uid msg)
+                      (MailServer.Deliver uid msg)
+| cm_delete uid msg :
+    compile_mail_base (Call (Mail.Delete uid msg))
+                      (MailServer.Delete uid msg)
+| cm_unlock uid :
+    compile_mail_base (Call (Mail.Unlock uid))
+                      (MailServer.Unlock uid)
+| cm_dataop {T} (op: Data.Op T) :
+    compile_mail_base (Call (Mail.DataOp op))
+                      (Call (DataOp op)).
+
+Definition mail_impl {gm: GoModel} :=
+  {| compile_rel_base := @compile_mail_base gm;
+     recover_rel := rec_singleton (MailServer.Recover) |}.
+
+Import Filesys.FS.
+Import GoLayer.Go.
+Import Mail.
+
+Definition init_base `{@GoModelWf gm} (s: GoLayer.Go.State) :=
+  s.(fs).(FS.heap) = ∅ ∧
+  (forall (uid: uint64),
+      (uid < 100 -> s.(fs).(dirents) !! (UserDir uid) = Some ∅) ∧
+      (uid >= 100 -> s.(fs).(dirents) !! (UserDir uid) = None)) ∧
+  s.(fs).(FS.dirents) !! SpoolDir = Some ∅ ∧
+  dom (gset string) s.(fs).(FS.dirents) =
+  dom (gset string) s.(fs).(FS.dirlocks) ∧
+  (∀ dir l, s.(fs).(FS.dirlocks) !! dir = Some l → fst l = Unlocked) ∧
+  s.(maillocks) = None.
+
+Definition init_absr `{@GoModelWf gm} sa sc := Mail.initP sa ∧ init_base sc.
+
+Lemma mail_crash_refinement_seq `{@GoModelWf gm} {T} σ1c σ1a esa esc:
+  init_absr σ1a σ1c →
+  wf_client_seq esa →
+  compile_rel_proc_seq mail_impl esa esc →
+  ¬ proc_exec_seq Mail.l esa (rec_singleton (Ret ())) (1, σ1a) Err →
+  ∀ σ2c (res: T), proc_exec_seq GoLayer.Go.l esc
+                                      (rec_singleton MailServer.Recover) (1, σ1c) (Val σ2c res) →
+  ∃ σ2a, proc_exec_seq Mail.l esa (rec_singleton (Ret tt)) (1, σ1a) (Val σ2a res).
+Proof.
+Abort.
